proof/invariants/findBlockInKS.v
@@ -1,0 +1,390 @@
+(*******************************************************************************)
+(*  © Université de Lille, The Pip Development Team (2015-2021)                *)
+(*                                                                             *)
+(*  This software is a computer program whose purpose is to run a minimal,     *)
+(*  hypervisor relying on proven properties such as memory isolation.          *)
+(*                                                                             *)
+(*  This software is governed by the CeCILL license under French law and       *)
+(*  abiding by the rules of distribution of free software.  You can  use,      *)
+(*  modify and/ or redistribute the software under the terms of the CeCILL     *)
+(*  license as circulated by CEA, CNRS and INRIA at the following URL          *)
+(*  "http://www.cecill.info".                                                  *)
+(*                                                                             *)
+(*  As a counterpart to the access to the source code and  rights to copy,     *)
+(*  modify and redistribute granted by the license, users are provided only    *)
+(*  with a limited warranty  and the software's author,  the holder of the     *)
+(*  economic rights,  and the successive licensors  have only  limited         *)
+(*  liability.                                                                 *)
+(*                                                                             *)
+(*  In this respect, the user's attention is drawn to the risks associated     *)
+(*  with loading,  using,  modifying and/or developing or reproducing the      *)
+(*  software by the user in light of its specific status of free software,     *)
+(*  that may mean  that it is complicated to manipulate,  and  that  also      *)
+(*  therefore means  that it is reserved for developers  and  experienced      *)
+(*  professionals having in-depth computer knowledge. Users are therefore      *)
+(*  encouraged to load and test the software's suitability as regards their    *)
+(*  requirements in conditions enabling the security of their systems and/or   *)
+(*  data to be ensured and,  more generally, to use and operate it in the      *)
+(*  same conditions as regards security.                                       *)
+(*                                                                             *)
+(*  The fact that you are presently reading this means that you have had       *)
+(*  knowledge of the CeCILL license and that you accept its terms.             *)
+(*******************************************************************************)
+
+(**  * Summary 
+    This file contains the invariants of [findBlockInKS, findBelongingBlock] and
+		associated lemmas.
+*)
+Require Import Model.Monad Model.Lib Model.MAL.
+Require Import Core.Internal.
+Require Import Proof.Consistency Proof.DependentTypeLemmas Proof.Hoare
+               Proof.Isolation Proof.StateLib Proof.WeakestPreconditions Proof.invariants.Invariants.
+Require Import Compare_dec Bool.
+
+Lemma findBlockComp  (entryaddr referenceaddr : paddr) (comparator : index) (P : state -> Prop)  : 
+{{fun s  =>  P s
+						/\ isBE entryaddr s}}
+Internal.findBlockComp entryaddr referenceaddr comparator
+{{fun isMatch s => P s}}.
+Proof.
+unfold Internal.findBlockComp.
+eapply bindRev.
+{ (** MAL.readBlockStartFromBlockEntryAddr *)
+	eapply weaken. apply readBlockStartFromBlockEntryAddr.
+	intros. simpl. split. apply H. intuition.
+}
+intro blockstart.
+eapply bindRev.
+{ (** MALInternal.Index.zero *)
+	eapply weaken. apply Index.zero.
+	intros. simpl. apply H.
+}
+intro zero. simpl.
+destruct beqIdx eqn:Hcomp.
+- (* beqIdx comparator zero = true *)
+	case_eq (beqAddr blockstart referenceaddr).
+	+ (* case_eq beqAddr blockstart referenceaddr = true *)
+		intros.
+		{ (** ret *)
+			eapply weaken. apply ret.
+			intros. simpl. apply H0.
+		}
+	+ (* case_eq beqAddr blockstart referenceaddr = false *)
+		intros.
+		{ (** ret *)
+			eapply weaken. apply ret.
+			intros. simpl. apply H0.
+		}
+- (* beqIdx comparator zero = false *)
+	eapply bindRev.
+	{ (** MAL.readBlockEndFromBlockEntryAddr *)
+		eapply weaken. apply readBlockEndFromBlockEntryAddr.
+		intros. simpl. split. apply H. intuition.
+	}
+	intro blockend.
+	eapply bindRev.
+	{ (** MALInternal.Paddr.leb *)
+		eapply weaken. apply Paddr.leb.
+		intros. simpl. apply H.
+	}
+	intro aboveStart.
+	eapply bindRev.
+	{ (** MALInternal.Paddr.leb *)
+		eapply weaken. apply Paddr.leb.
+		intros. simpl. apply H.
+	}
+	intro belowEnd.
+	case_eq (aboveStart && belowEnd).
+	+ (* case_eq aboveStart && belowEnd = true *)
+		intros.
+		{ (** ret *)
+			eapply weaken. apply ret.
+			intros. simpl. apply H0.
+		}
+	+ (* case_eq aboveStart && belowEnd = false *)
+		intros.
+		{ (** ret *)
+			eapply weaken. apply ret.
+			intros. simpl. apply H0.
+		}
+Qed.
+
+Lemma findBlockInKSInStructAux n (currentidx : index)
+																(currentkernelstructure referenceaddr : paddr)
+																(compoption : index) (P : state -> Prop) :
+{{  fun s : state => P s /\ consistency s
+										/\ isKS currentkernelstructure s
+										/\ currentidx < kernelStructureEntriesNb
+										/\ currentidx < maxIdx -1
+}}
+Internal.findBlockInKSInStructAux n currentidx currentkernelstructure referenceaddr compoption
+{{fun (blockaddr : paddr) (s : state) => P s /\ consistency s /\
+		(blockaddr = nullAddr
+				\/ (exists entry, lookup blockaddr s.(memory) beqAddr = Some (BE entry)))
+}}.
+Proof.
+(* revert mandatory to generalize the induction hypothesis *)
+revert currentidx currentkernelstructure referenceaddr compoption.
+induction n.
+- (* n = 0 *)
+	intros;simpl.
+	{	(* MALInternal.getNullAddr *)
+		eapply weaken. unfold MALInternal.getNullAddr.
+		eapply WP.ret. intros. simpl. intuition.
+	}
+- (* n = S n*)
+	(*unfold Internal.findBlockInKSInStructAux.*)
+	intros.
+	eapply bindRev.
+	{ (** getBlockEntryAddrFromKernelStructureStart *)
+		eapply weaken. apply getBlockEntryAddrFromKernelStructureStart.
+		intros. split. apply H. unfold consistency in *. cbn. intuition.
+	}
+	intro entryaddr.
+	eapply bindRev.
+	{ (** MAL.readBlockPresentFromBlockEntryAddr *)
+		eapply weaken. apply readBlockPresentFromBlockEntryAddr.
+		intros. simpl. split. apply H. intuition.
+	}
+	intro ispresent.
+	eapply bindRev.
+	{ (** findBlockComp *)
+		eapply weaken. apply findBlockComp.
+		intros. simpl. split. apply H. intuition.
+	}
+	intro matchcomp.
+	case_eq (ispresent && matchcomp).
+	+ (* case_eq ispresent && matchcomp = true *)
+		intros.
+		{ (** ret *)
+			eapply weaken. apply ret.
+			intros. simpl. intuition. right. apply isBELookupEq. intuition.
+		}
+	+ (* case_eq ispresent && matchcomp = false *)
+		intros.
+		eapply bindRev.
+		{ (** getKernelStructureEntriesNb *)
+			eapply weaken. apply getKernelStructureEntriesNb.
+			intros. simpl. apply H0.
+		}
+		intro maxentriesnb.
+		eapply bindRev.
+		{ (** succ *)
+			eapply weaken. apply Index.succ.
+			intros. simpl. split. apply H0. intuition.
+			(*apply PeanoNat.Nat.lt_add_lt_sub_l.
+			apply PeanoNat.Nat.lt_add_lt_sub_l in H8.
+			rewrite KSEntriesNbLessThanMaxIdx in *. assumption.*)
+		}
+		intro nextidx.
+		eapply bindRev.
+		{ (** Index.ltb *)
+			eapply weaken. apply Index.ltb.
+			intros. simpl. apply H0.
+		}
+		intro isnotlastidx.
+		case_eq (isnotlastidx).
+		* (* case_eq isnotlastidx = true *)
+			intros.
+			{ (** induction hypothesis *)
+				eapply weaken. apply IHn.
+				intros. intuition.
+				- unfold StateLib.Index.ltb in *.
+					apply eq_sym in H3.
+					apply PeanoNat.Nat.ltb_lt in H3. subst.
+					unfold CIndex in *.
+					destruct (lt_dec kernelStructureEntriesNb maxIdx).
+					intuition. contradict n0. rewrite KSEntriesNbLessThanMaxIdx. intuition.
+				- (* nextidx < kernelStructureEntriesNb < maxIdx - 1*)
+					unfold StateLib.Index.succ in *.
+					destruct (lt_dec (currentidx + 1) maxIdx) ; try (exfalso ; congruence).
+					destruct nextidx. simpl in *.
+					unfold StateLib.Index.ltb in *.
+					apply eq_sym in H3.
+					apply PeanoNat.Nat.ltb_lt in H3. subst.
+					unfold CIndex in *.
+					destruct (lt_dec kernelStructureEntriesNb maxIdx).
+					simpl in *. intuition.
+					contradict n0. rewrite KSEntriesNbLessThanMaxIdx. intuition.
+		}
+		* (* case_eq isnotlastidx = false *)
+			intros.
+			{ (** ret *)
+				eapply weaken. apply ret.
+				intros. simpl. intuition.
+			}
+Qed.
+
+Lemma findBlockInKSAux n (currentkernelstructure idblock : paddr) 
+																(compoption : index) (P : state -> Prop) :
+{{  fun s : state => P s /\ consistency s
+										/\ isKS currentkernelstructure s}}
+Internal.findBlockInKSAux n currentkernelstructure idblock compoption
+{{fun (blockaddr : paddr) (s : state) => P s /\ consistency s /\
+																				(blockaddr = nullAddr \/
+																	(exists entry, lookup blockaddr s.(memory) beqAddr = Some (BE entry)
+																			(*/\ blockaddr = idblock*))) }}.
+Proof.
+(* revert mandatory to generalize the induction hypothesis *)
+revert currentkernelstructure idblock compoption.
+induction n.
+- (* n = 0 *)
+	intros;simpl.
+	(* MALInternal.getNullAddr *)
+	eapply weaken. unfold MALInternal.getNullAddr.
+	eapply WP.ret. intros. simpl. intuition.
+- (* n = S n*)
+	unfold Internal.findBlockInKSAux.
+	intros.
+	eapply bindRev.
+	{ (** MALInternal.Index.zero *)
+		eapply weaken. apply Index.zero.
+		intros. simpl. apply H.
+	}
+	intro zero.
+	eapply bindRev.
+	{ (** Internal.findBlockInKSInStructAux *)
+		eapply weaken. apply findBlockInKSInStructAux.
+		intros. simpl. split. apply H. intuition.
+		- (* zero < kernelStructureEntriesNb by axiom *)
+			apply CIndex0ltKSEntriesNb. assumption.
+		- (* zero < maxIdx - 1 by axiom *)
+			apply CIndex0ltMaxIdx. assumption.
+	}
+	intro foundblock.
+	eapply bindRev.
+	{ (** Internal.compareAddrToNull *)
+		eapply weaken. apply compareAddrToNull.
+		intros. simpl. apply H.
+	}
+	intro foundblockisnull.
+	case_eq foundblockisnull.
+	+ (* case_eq foundblockisnull = true *)
+		intros.
+		eapply bindRev.
+		{ (** MAL.readNextFromKernelStructureStart *)
+			eapply weaken. apply readNextFromKernelStructureStart.
+			intros. simpl. split. apply H0. unfold consistency in *. intuition.
+		}
+		intro nextkernelstructure.
+		eapply bindRev.
+		{ (** Internal.compareAddrToNull *)
+			eapply weaken. apply compareAddrToNull.
+			intros. simpl. apply H0.
+		}
+		intro nextKSisnull.
+		case_eq nextKSisnull.
+		* (* case_eq nextKSisnull = true *)
+			intros.
+		{ (** ret *)
+			eapply weaken. apply ret.
+			intros. simpl. intuition.
+		}
+		* (* case_eq nextKSisnull = false *)
+			intros.
+			{ (** induction hypothesis *)
+				eapply weaken. apply IHn.
+				intros. simpl. split. apply H1. split. apply H1. intuition.
+				- destruct H4. unfold consistency in *. intuition.
+				unfold NextKSIsKS in *.
+				apply beqAddrFalse in H3.
+				eauto.
+				- (* impossible, foundblock is null *)
+					contradict H9.
+					apply beqAddrTrue in H5. subst.
+					unfold consistency in *.
+					unfold nullAddrExists in *.
+					intuition. unfold isPADDR in *.
+					destruct H.
+					rewrite H in *. congruence.
+			}
+	+ (* case_eq foundblockisnull = false *)
+		intros. simpl.
+		{ (** ret *)
+			eapply weaken. apply ret.
+			intros. simpl. intuition.
+		}
+Qed.
+
+Lemma findBelongingBlock (idPD referenceaddr: paddr) (P : state -> Prop) :
+{{ fun s => P s /\ consistency s /\ isPDT idPD s}}
+Internal.findBelongingBlock idPD referenceaddr 
+{{fun (blockaddr : paddr) (s : state) => P s /\ consistency s /\
+			(blockaddr = nullAddr
+					\/ (exists entry, lookup blockaddr s.(memory) beqAddr = Some (BE entry)
+																			(*/\ blockaddr = blockEntryAddr*)))
+}}.
+Proof.
+unfold Internal.findBelongingBlock.
+eapply bindRev.
+{ (** MALInternal.Index.zero *)
+	eapply weaken. apply Index.zero.
+	intros. simpl. apply H.
+}
+intro zero.
+eapply bindRev.
+{ (** MALInternal.Index.succ *)
+	eapply weaken. apply Index.succ.
+	intros. simpl. split. apply H.
+	intuition. rewrite H1. unfold CIndex. destruct (lt_dec 0 maxIdx).
+	simpl. rewrite <- PeanoNat.Nat.lt_add_lt_sub_l.
+	simpl. apply maxIdxBigEnough.
+	contradict n. apply maxIdxNotZero.
+}
+intro one.
+eapply bindRev.
+{ (** MAL.readPDStructurePointer *)
+	eapply weaken. apply readPDStructurePointer.
+	intros. simpl. split. apply H. intuition.
+}
+intro kernelstructurestart.
+{ (** Internal.findBlockInKSAux *)
+	eapply weaken. apply findBlockInKSAux.
+	intros. simpl. intuition.
+	unfold pdentryPDStructurePointer in *.
+	unfold isPDT in *.
+	destruct (lookup idPD (memory s) beqAddr) eqn:Hlookup ; try (exfalso ; congruence).
+	destruct v eqn:Hv ; try (exfalso ; congruence).
+	unfold consistency in *.
+	unfold StructurePointerIsKS in *. intuition.
+	subst.
+	apply H16 with idPD. assumption.
+}
+Qed.
+
+Lemma findBlockInKS (idPD blockEntryAddr: paddr) (P : state -> Prop) :
+{{ fun s => P s /\ consistency s /\ isPDT idPD s}}
+Internal.findBlockInKS idPD blockEntryAddr 
+{{fun (blockaddr : paddr) (s : state) => P s /\ consistency s /\
+			(blockaddr = nullAddr
+					\/ (exists entry, lookup blockaddr s.(memory) beqAddr = Some (BE entry)
+																			(*/\ blockaddr = blockEntryAddr*)))
+}}.
+Proof.
+unfold Internal.findBlockInKS.
+eapply bindRev.
+{ (** MALInternal.Index.zero *)
+	eapply weaken. apply Index.zero.
+	intros. simpl. apply H.
+}
+intro zero.
+eapply bindRev.
+{ (** MAL.readPDStructurePointer *)
+	eapply weaken. apply readPDStructurePointer.
+	intros. simpl. split. apply H. intuition.
+}
+intro kernelstructurestart.
+{ (** Internal.findBlockInKSAux *)
+	eapply weaken. apply findBlockInKSAux.
+	intros. simpl. intuition.
+	unfold pdentryPDStructurePointer in *.
+	unfold isPDT in *.
+	destruct (lookup idPD (memory s) beqAddr) eqn:Hlookup ; try (exfalso ; congruence).
+	destruct v eqn:Hv ; try (exfalso ; congruence).
+	unfold consistency in *.
+	unfold StructurePointerIsKS in *. intuition.
+	subst.
+	apply H15 with idPD. assumption.
+}
+Qed.
+
