proof/invariants/getGlobalIdPDCurrentOrChild.v
@@ -31,80 +31,78 @@
 (*  knowledge of the CeCILL license and that you accept its terms.             *)
 (*******************************************************************************)
 
-(** * Summary 
-    This file contains the invariant of [checkChildOfCurrPart].
+(** * Summary
+    This file contains the invariant of [getGlobalIdPDCurrentOrChild].
 *)
-Require Import Model.Monad Model.Lib Model.MAL.
-Require Import Core.Internal.
-Require Import Proof.Consistency Proof.DependentTypeLemmas Proof.Hoare
-               Proof.Isolation Proof.StateLib Proof.WeakestPreconditions Proof.invariants.Invariants
-							 Proof.invariants.findBlockInKSWithAddr.
 
-Lemma checkChildOfCurrPart (currentPartition idPDchild : paddr) P :
-{{ fun s => P s /\ consistency s /\ isPDT currentPartition s}}
-Internal.checkChildOfCurrPart  currentPartition idPDchild
-{{fun isChild s => P s
-/\ (isChild = true -> exists sh1entryaddr, isChild = StateLib.checkChild idPDchild s sh1entryaddr
-										/\ exists entry, lookup idPDchild s.(memory) beqAddr = Some (BE entry)
-										/\ exists sh1entry, lookup sh1entryaddr s.(memory) beqAddr = Some (SHE sh1entry))
-}}.
+Require Import Model.ADT Core.Services Model.MALInternal Model.Lib.
+Require Import Proof.Isolation Proof.Hoare Proof.Consistency Proof.WeakestPreconditions
+Proof.StateLib Proof.DependentTypeLemmas.
+Require Import invariants.Invariants invariants.checkChildOfCurrPart.
+
+Require Import Model.Monad (* for visibility *).
+
+Module WP := WeakestPreconditions.
+
+Lemma getGlobalIdPDCurrentOrChild (currentPartition idPDToCheck : paddr) (P : state -> Prop):
+{{fun s => P s /\ consistency s
+					/\ isPDT currentPartition s}}
+Internal.getGlobalIdPDCurrentOrChild currentPartition idPDToCheck
+{{fun idPDChild s  => P s /\ consistency s /\
+										(idPDChild <> nullAddr -> isPDT idPDChild s) }}.
 Proof.
-unfold Internal.checkChildOfCurrPart.
-eapply WP.bindRev.
-{
-	(** findBlockInKSWithAddr *)
-	eapply weaken. apply findBlockInKSWithAddr.
-	intros. simpl. split. apply H. intuition.
-}
-intro blockInParentPartAddr. simpl.
-(** compareAddrToNull **)
-eapply WP.bindRev.
-{
-	eapply weaken. eapply compareAddrToNull.
+unfold Internal.getGlobalIdPDCurrentOrChild.
+eapply bindRev.
+{ (** MALInternal.getBeqAddr **)
+	eapply weaken. apply getBeqAddr.
 	intros. simpl. apply H.
 }
-intro addrIsNull0.
-simpl.
-case_eq addrIsNull0.
-- (* case_eq addrIsNull0 = true*)
+intro isCurrentPart.
+case_eq isCurrentPart.
+- (* case_eq isCurrentPart = true *)
+	intros.
 	{ (** ret *)
-		intros. eapply WP.weaken. apply WP.ret.
-		intros. simpl. intuition.
+	eapply weaken. apply WP.ret.
+  simpl. intros. intuition.
 	}
-- (* case_eq addrIsNull0 = false *)
+- (* case_eq isCurrentPart = false *)
 	intros.
 	eapply bindRev.
-	{	(** Invariants.readSh1PDFlagFromBlockEntryAddr *)
-		eapply weaken. apply Invariants.readSh1PDFlagFromBlockEntryAddr.
-		intros. simpl. split. apply H0.
-		intuition.
-		intros. simpl.
-		(* prove blockInParentPartAddr can't be NULL and not NULL at the same time *)
-		apply beqAddrFalse in H2. exfalso ; congruence.
-		destruct H4. exists x. apply H4.
+	{ (** Internal.checkChildOfCurrPart *)
+		eapply weaken. apply checkChildOfCurrPart.
+		intros. simpl. split. apply H0. intuition.
 	}
-		intro isChild. simpl.
-		case_eq isChild.
-		+ (* ischild =  true *)
-			intro childIsNotNull. simpl.
-			{ (** ret *)
-				eapply weaken. apply WP.ret.
-				intros. simpl. intuition.
-				(*blockInParentPartAddr can't be NULL and not NULL at the same time *)
-				apply beqAddrFalse in H3. exfalso ; congruence.
-				destruct H2. destruct H2. exists x0.
-				split. unfold checkChild. destruct H5. intuition. subst. 
-				rewrite H2. rewrite H8.
-				unfold sh1entryPDflag in *. rewrite -> H8 in *. assumption.
-				destruct H5. exists x1. split. intuition. subst. assumption.
-				exists x. intuition.
-			}
-	 	+ (* ischild = false : sh1entry exists but PDflag = 0 *)
-			simpl. intros.
-			{ (** ret *)
-				eapply weaken. apply WP.ret.
-				intros. simpl. split. apply H1.
-				intuition.
-			}
+	intro isChildCurrPart.
+	case_eq isChildCurrPart.
+	+ (* case_eq isChildCurrPart = true *)
+		intros.
+		eapply bindRev.
+		{ (** MAL.readBlockStartFromBlockEntryAddr *)
+			eapply weaken. apply readBlockStartFromBlockEntryAddr.
+			intros. simpl. split. apply H1. intuition.
+			destruct H5. intuition. destruct H7.
+			unfold isBE. intuition. rewrite H7 ; trivial.
+		}
+		intro idPDChild.
+		{ (** ret *)
+		eapply weaken. apply WP.ret.
+		simpl. intros. intuition.
+		destruct H6. unfold consistency in *. unfold PDTIfPDFlag in *.
+		intuition. unfold entryPDT in *. destruct H10. intuition.
+		specialize (H6 idPDToCheck x H2).
+		destruct H6. intuition.
+		unfold bentryStartAddr in *. rewrite H10 in *. subst.
+		unfold isPDT.
+		destruct (lookup (startAddr (blockrange x1)) (memory s) beqAddr) eqn:Hlookup ; try (exfalso ; congruence).
+		destruct v eqn:Hv ; try (exfalso ; congruence) ; trivial.
+		}
+	+ (* case_eq isChildCurrPart = false *)
+		intros.
+		{ (** ret *)
+		eapply weaken. apply WP.ret.
+		simpl. intros. intuition.
+		}
 Qed.
+
+
 
